Add IPM lecture Coq file

go/heap/heap.go
@@ -1,7 +1,25 @@
 package heap
 
+import "github.com/goose-lang/primitive"
+
 func Swap(x *uint64, y *uint64) {
 	old_y := *y
 	*y = *x
 	*x = old_y
+}
+
+// IgnoreOneLocF has a specification that shows it does not need ownership of
+// its second argument.
+func IgnoreOneLocF(x *uint64, y *uint64) {
+	primitive.Assert(*x == 0)
+	*x = 42
+}
+
+// UseIgnoreOneLocOwnership uses IgnoreOneLocF and can be verified using its
+// specification.
+func UseIgnoreOneLocOwnership() {
+	var x = uint64(0)
+	var y = uint64(42)
+	IgnoreOneLocF(&x, &y)
+	primitive.Assert(x == y)
 }
