src/sys_verif/program_proof/empty_ffi.v
@@ -1,0 +1,34 @@
+From Perennial.goose_lang Require Import lang lifting typing.
+
+#[export] Instance empty_ext : ffi_syntax :=
+  {| ffi_opcode := Empty_set;
+     ffi_val := Empty_set;
+  |}.
+
+#[export] Instance empty_model : ffi_model :=
+  {| ffi_state := unit;
+     ffi_global_state := unit;
+  |}.
+
+#[export] Instance empty_ffi_interp : ffi_interp empty_model :=
+    {| ffiLocalGS := λ _, unit;
+       ffiGlobalGS _ := unit;
+       ffi_local_ctx Σ _ (d: @ffi_state empty_model) := True%I;
+       ffi_global_ctx _ _ _ := True%I;
+       ffi_local_start Σ _ (d: @ffi_state empty_model) := True%I;
+       ffi_global_start _ _ _ := True%I;
+       ffi_restart := fun _ _ (d: @ffi_state empty_model) => True%I;
+       ffi_crash_rel Σ hF1 σ1 hF2 σ2 := True%I;
+    |}.
+
+#[export] Instance empty_semantics : ffi_semantics empty_ext empty_model :=
+  {| ffi_step := λ op v, Transitions.runF (λ s, (s, Val v));
+    ffi_crash_step := λ _ _, True |}.
+
+#[export] Instance empty_val_ty : val_types :=
+  {| ext_tys :=  Empty_set; |}.
+
+#[export] Instance empty_types : ext_types empty_ext :=
+  {| val_tys := empty_val_ty;
+    get_ext_tys := λ v '(t1, t2), True;
+  |}.
