go/go.mod
@@ -3,6 +3,7 @@ module sys_verif_code
 go 1.22
 
 require (
+	github.com/goose-lang/primitive v0.1.0
 	github.com/goose-lang/std v0.5.0
 	github.com/stretchr/testify v1.9.0
 	pgregory.net/rapid v1.1.0
@@ -10,7 +11,6 @@ require (
 
 require (
 	github.com/davecgh/go-spew v1.1.1 // indirect
-	github.com/goose-lang/primitive v0.1.0 // indirect
 	github.com/pmezard/go-difflib v1.0.0 // indirect
 	gopkg.in/yaml.v3 v3.0.1 // indirect
 )
